Prove ayclicity of HeadRewire

uniana/cfg/HeadRewire.v
@@ -1,10 +1,12 @@
-Require Export CFGinnermost CFGgeneral.
+Require Export CFGinnermost CFGgeneral EEdge.
 
 Section hr_cfg.
   Context `{C : redCFG}.
 
   Definition head_rewired_edge q p : Prop
     := edge__P q p /\ ~ loop_head q \/ exited q p.
+
+  Infix "-h>" := (head_rewired_edge) (at level 70).
 
   Lemma subgraph_refl {L : Type} [edge1 : L -> L -> Prop]
     : sub_graph edge1 edge1.
@@ -51,6 +53,40 @@ Section hr_cfg.
         * destruct H0. eapply deq_loop_exited' in H0. eapply H0 in Hloop. contradiction.
   Qed.
 
+  Lemma head_rewired_cycle_not_contains p q t
+        (Hpath : HPath p q t)
+        (Hedge : q -h> p) x y
+        (Hinx : x ∈ t)
+        (Hiny : y ∈ t)
+        (Hloop : loop_contains x y)
+    : x = y.
+  Proof.
+    eapply in_split in Hinx as Hsplitx.
+    destructH.
+    rewrite Hsplitx in Hiny.
+    eapply in_app_or in Hiny.
+    cbn in Hiny.
+    eapply path_postfix_path in Hpath as Hx;eauto.
+    2: { rewrite postfix_eq. setoid_rewrite <-app_cons_assoc. exists l2. eassumption. }
+    destruct Hiny as [Hiny|[Hiny|Hiny]];[|assumption|].
+    - eapply in_split in Hiny as Hsplity.
+      destructH.
+      eapply path_prefix_path in Hpath as Hy;eauto.
+      2: { eapply prefix_eq. exists l0. rewrite Hsplity in Hsplitx. rewrite <-app_assoc in Hsplitx.
+           cbn in Hsplitx. eassumption.
+      }
+      eapply head_rewired_head_no_entry;eauto.
+      eapply path_app;eauto.
+    - eapply in_split in Hiny as Hsplity.
+      destructH.
+      eapply path_prefix_path in Hpath as Hy;eauto.
+      2: { eapply prefix_eq. exists (l1 ++ x :: l0). rewrite Hsplity in Hsplitx.
+           rewrite <-app_assoc. cbn. eassumption.
+      }
+      eapply head_rewired_head_no_entry;eauto.
+      eapply path_app;eauto.
+  Qed.
+
   Lemma head_rewired_entry_eq h p q t
         (Hpath : HPath q p t)
         (Hnin : ~ loop_contains h q)
@@ -69,25 +105,176 @@ Section hr_cfg.
         * destruct H0. eapply deq_loop_exited' in H0. eapply H0 in Hin. contradiction.
   Qed.
 
+  Definition loop_contains_strict h p
+    := loop_contains h p /\ h <> p.
+
+  Definition deq_loop_mh q p
+    := forall h, h <> p -> loop_contains h p -> loop_contains h q.
+
+  Definition eq_loop_mh q p
+    := deq_loop_mh q p /\ deq_loop_mh p q.
+
+  Lemma eq_loop_mh_sym : Symmetric eq_loop_mh.
+  Proof.
+    firstorder.
+  Qed.
+
+  Instance deq_loop_mh_refl : Reflexive deq_loop_mh.
+  Proof.
+    unfold Reflexive. intros x h Hloop Hneq.
+    auto.
+  Qed.
+
+  Lemma deq_loop_deq_loop_mh p q
+        (Hdeq : deq_loop p q)
+    : deq_loop_mh p q.
+  Proof.
+    intros h Hloop Hneq.
+    eauto.
+  Qed.
+
+  Lemma deq_loop_mh_deq_loop p q
+        (Hnh : ~ loop_head q)
+        (Hdeq : deq_loop_mh p q)
+    : deq_loop p q.
+  Proof.
+    intros h Hloop.
+    eapply Hdeq.
+    - contradict Hnh. subst h. eapply loop_contains_loop_head;eauto.
+    - assumption.
+  Qed.
+
+  Lemma head_rewired_deq_loop_mh p q
+        (Hedge : p -h> q)
+  : deq_loop_mh p q.
+  Proof.
+    destruct Hedge.
+    - destructH. destruct (edge_Edge H0);intros h Hloop Hneq.
+      + eapply basic_edge_eq_loop in b.
+        rewrite b. auto.
+      + eapply back_edge_eq_loop in b. rewrite b. assumption.
+      + eapply deq_loop_entry_or in e;eauto.
+        destruct e;[assumption|contradiction].
+      + destruct e. eapply deq_loop_exited;eauto.
+    - destruct H. intros h Hloop Hneq.
+      eapply deq_loop_exited';eauto.
+  Qed.
+
+  Lemma hpath_deq_loop_mh p q π
+        (Hpath : HPath p q π)
+    : deq_loop_mh p q.
+  Proof.
+    induction Hpath.
+    - reflexivity.
+    - eapply head_rewired_deq_loop_mh in H as Hmh.
+      intros h Hneq Hloop.
+      eapply IHHpath;eauto.
+      contradict Hloop.
+      subst h. eapply head_rewired_not_contains;eauto.
+  Qed.
+
+  Lemma hpath_deq_loop_mh_elem p q π x
+        (Hpath : HPath p q π)
+        (Hin : x ∈ π)
+    : deq_loop_mh x q.
+  Proof.
+    eapply path_from_elem in Hpath;eauto.
+    destructH.
+    eapply hpath_deq_loop_mh;eauto.
+  Qed.
+
+  Lemma rotate_forward' (L : Type) (e : L -> L -> Prop) (p q : L) π
+        (Hedge : e q p)
+        (Hpath : Path e p q π)
+    : let π' := p :: r_tl π in
+      let q' := hd p (rev π') in
+      e p q' /\ Path e q' p π'.
+  Proof.
+    intros. subst q' π'. cbn.
+      destr_r' π;subst;cbn.
+      1: inv Hpath.
+      rewrite r_tl_rcons.
+      Lemma hd_rcons' (A : Type) (a : A) (l : list A)
+        : hd a (l ++ [a]) = hd a l.
+      Proof.
+        induction l;cbn;eauto.
+      Qed.
+      rewrite hd_rcons'. path_simpl' Hpath.
+      destr_r' l;subst;cbn in *.
+      + path_simpl' Hpath. split; assumption.
+      + rewrite rev_rcons. cbn.
+        split.
+        * eapply path_nlrcons_edge in Hpath;eauto.
+        * eapply path_rcons_rinv in Hpath. econstructor;eauto.
+  Qed.
+
+  Lemma rotate_forward (L : Type) (e : L -> L -> Prop) (p q : L) π
+        (Hedge : e q p)
+        (Hpath : Path e p q π)
+    : exists π' q', e p q' /\ Path e q' p π'.
+  Proof.
+    do 2 eexists;eapply rotate_forward';eauto.
+  Qed.
+
+  Lemma loop_reachs_exit h p q
+        (Hexit : exit_edge h p q)
+    : h -a>* q.
+  Proof.
+    copy Hexit Hexit'.
+    destruct Hexit.
+    eapply loop_reachs_member in H.
+    destruct H.
+    exists (q :: x).
+    econstructor;eauto.
+    eapply exit_a_edge;eauto.
+  Qed.
+
   Lemma acyclic_head_rewired_edge
     : acyclic head_rewired_edge.
   Proof.
-    eapply acyclic_path_path;eauto.
-    2: { intros. intro. subst. eapply head_rewired_no_self;eauto. }
-    intros p q π. revert p q. induction π;intros p q ϕ Hneq Hπ Hϕ;inv_path Hπ.
-    - contradiction.
-    - decide (p = x).
-      + subst x.
-        eapply IHπ in H.
-(*
-    unfold acyclic. intros.
-    revert p q H H0. induction π;intros p q Hedge Hpath;inv_path Hpath.
-    - destruct Hedge.
-      + destruct H. eapply no_self_loops;eauto.
-      + destruct H. destruct H. destruct H0. eapply H0.
-        eauto using loop_contains_self,loop_contains_loop_head.
-    - *)
-  Admitted.
+    intros p q π Hedge Hpath.
+    specialize (head_rewired_cycle_not_contains) with (p:=q) (q:=p) (t:=π) as Hnl.
+    do 2 exploit' Hnl.
+    enough (q -a>* p) as Hacy.
+    {
+      destruct Hedge.
+      - destruct Hacy.
+        eapply a_edge_acyclic;eauto.
+        destruct H.
+        decide (back_edge p q).
+        + exfalso. eapply loop_contains_ledge in b. eapply Hnl in b.
+          * subst. eapply no_self_loops;eauto.
+          * eapply path_contains_back;eauto.
+          * eapply path_contains_front;eauto.
+        + do 2 simpl_dec' n. destruct n;firstorder.
+      - copy H Hexit.
+        destruct Hexit as [pq Hexit].
+        eapply loop_reachs_exit in Hexit.
+        destruct Hacy. destruct Hexit.
+        inv_path H0.
+        + eapply head_rewired_no_self;right;eauto.
+        + eapply a_edge_acyclic;eauto.
+          eapply path_app';eauto.
+    }
+    clear Hedge.
+    induction Hpath.
+    - eexists;econstructor.
+    - exploit IHHpath. destruct IHHpath.
+      destruct H.
+      + exists (c :: x).
+        econstructor;eauto.
+        decide (back_edge b c). 2: { destruct H. do 2 simpl_dec' n. destruct n;[contradiction|auto]. }
+        exfalso.
+        eapply loop_contains_ledge in b0.
+        eapply Hnl in b0. 2: auto. 2: right;eapply path_contains_front;eauto.
+        subst.
+        eapply head_rewired_no_self. left;eauto.
+      +
+        destruct H.
+        eapply loop_reachs_exit in H. destruct H.
+        eexists.
+        eapply path_app';eauto.
+  Qed.
 
   Lemma acyclic_HPath p q π
         (Hpath : HPath p q π)
